\documentclass{article}
\usepackage{amsmath}
\usepackage{amssymb}

\title{Application of the Cauchy-Schwarz Inequality and the Arithmetic-Geometric Mean Inequality}
\author{mxsail,\\Intermediate Algebra,\\Art of Problem Solving}
\date{\today}

\begin{document}
\maketitle

\section*{Problem Statement}
\begin{enumerate}
    \item[(a)] Show that if $a,$ $b,$ $c,$ $d,$ $e,$ $f$ are nonnegative real numbers, then
    \[
    (a^2 + b^2)^2 (c^4 + d^4)(e^4 + f^4) \ge (ace + bdf)^4.
    \]
    \item[(b)] Show that if $a,$ $b,$ $c,$ $d,$ $e,$ $f$ are nonnegative real numbers, then
    \[
    (a^2 + b^2)(c^2 + d^2)(e^2 + f^2) \ge (ace + bdf)^2.
    \]
\end{enumerate}

\section*{Solution}
Both parts of the problem can be solved using the Cauchy-Schwarz inequality and the Arithmetic-Geometric Mean (AM-GM) inequality.

\subsection*{Part (a)}
We begin by applying the Cauchy-Schwarz inequality:
\[
(c^4 + d^4)(e^4 + f^4) \ge (c^2e^2 + d^2f^2)^2.
\]
Multiplying both sides by $(a^2 + b^2)^2$ gives:
\[
(a^2 + b^2)^2(c^4 + d^4)(e^4 + f^4) \ge (a^2 + b^2)^2(c^2e^2 + d^2f^2)^2.
\]
Now we expand the right-hand side:
\[
(a^2 + b^2)^2(c^2e^2 + d^2f^2)^2 = \left(a^2c^2e^2 + a^2d^2f^2 + b^2c^2e^2 + b^2d^2f^2\right)^2.
\]

Let us group the terms:
\[
\left(a^2c^2e^2 + b^2d^2f^2 + a^2d^2f^2 + b^2c^2e^2\right)^2.
\]

Apply AM-GM to the middle two terms:
\[
a^2d^2f^2 + b^2c^2e^2 \ge 2\sqrt{a^2d^2f^2 \cdot b^2c^2e^2} = 2abcdef.
\]
Hence,
\[
\left(a^2c^2e^2 + b^2d^2f^2 + 2abcdef\right)^2 \ge (ace + bdf)^4.
\]

Thus, we conclude:
\[
(a^2 + b^2)^2(c^4 + d^4)(e^4 + f^4) \ge (ace + bdf)^4.
\]

\subsection*{Part (b)}
We expand the left-hand side:
\begin{align*}
&(a^2 + b^2)(c^2 + d^2)(e^2 + f^2) = \\
&\quad a^2c^2e^2 + a^2c^2f^2 + a^2d^2e^2 + a^2d^2f^2 + b^2c^2e^2 + b^2c^2f^2 + b^2d^2e^2 + b^2d^2f^2.
\end{align*}

Group $a^2c^2e^2$ and $b^2d^2f^2$ separately. Apply AM-GM to the remaining six terms:
\[
a^2c^2f^2 + a^2d^2e^2 + a^2d^2f^2 + b^2c^2e^2 + b^2c^2f^2 + b^2d^2e^2 \ge 6\sqrt[6]{(a^2b^2c^4d^4e^4f^4)} = 6abcdef.
\]

So the total expression satisfies:
\[
(a^2 + b^2)(c^2 + d^2)(e^2 + f^2) \ge a^2c^2e^2 + b^2d^2f^2 + 6abcdef.
\]

Now, observe that:
\[
a^2c^2e^2 + b^2d^2f^2 + 6abcdef \ge (ace + bdf)^2,
\]
since
\[
(ace + bdf)^2 = a^2c^2e^2 + b^2d^2f^2 + 2abcdef \le a^2c^2e^2 + b^2d^2f^2 + 6abcdef.
\]

Therefore, we conclude:
\[
(a^2 + b^2)(c^2 + d^2)(e^2 + f^2) \ge (ace + bdf)^2.
\]

\end{document}
