\documentclass{article}
\usepackage{amsmath}
\usepackage{amssymb}

\title{Week 18 Writing Problem}
\author{mxsail}
\date{\today}

\begin{document}

\maketitle

\section*{Problem Statment}
Let
\[f(x) = \frac{x - \sqrt{3}}{x\sqrt{3} + 1}.\]What is $f^{2012}(x)$, where the function is being applied $2012$ times?
This notation indicates repeated composition of functions, not exponentiation of functions. For example,\[f^2(x)=f(f(x))\]and not $f(x) \cdot f(x).$ Similarly,\[f^3(x)=f(f(f(x))).\]

\section*{Solution}
The key observation is to note that $f(x)$ is a MÃ¶bius transformation, and repeated application of $f$ can be analyzed by studying its properties.

Let us compute the first few iterations:
\[
f(x) = \frac{x - \sqrt{3}}{x\sqrt{3} + 1}
\]
\[
f^2(x) = f(f(x)) = \frac{f(x) - \sqrt{3}}{f(x)\sqrt{3} + 1}
\]
Substitute $f(x)$:
\[
f^2(x) = \frac{\frac{x - \sqrt{3}}{x\sqrt{3} + 1} - \sqrt{3}}{\frac{x - \sqrt{3}}{x\sqrt{3} + 1}\sqrt{3} + 1}
\]
\begin{align*}
&\frac{x - \sqrt{3} - \sqrt{3}(x\sqrt{3} + 1)}{x\sqrt{3} + 1} \\
&= \frac{x - \sqrt{3} - x\cdot 3 - \sqrt{3}}{x\sqrt{3} + 1} \\
&= \frac{x - 3x - \sqrt{3} - \sqrt{3}}{x\sqrt{3} + 1} \\
&= \frac{-2x - 2\sqrt{3}}{x\sqrt{3} + 1}
\end{align*}
Simplify denominator:
\[
\frac{(x - \sqrt{3})\sqrt{3}}{x\sqrt{3} + 1} + 1
= \frac{x\sqrt{3} - 3}{x\sqrt{3} + 1} + 1
= \frac{x\sqrt{3} - 3 + x\sqrt{3} + 1}{x\sqrt{3} + 1}
= \frac{2x\sqrt{3} - 2}{x\sqrt{3} + 1}
\]
So,
\[
f^2(x) = \frac{-2(x + \sqrt{3})}{2(x\sqrt{3} - 1)} = -\frac{x + \sqrt{3}}{x\sqrt{3} - 1}
\]

Now, compute $f^3(x)$:
\[
f^3(x) = f(f^2(x)) = \frac{f^2(x) - \sqrt{3}}{f^2(x)\sqrt{3} + 1}
\]
Let $y = f^2(x) = -\frac{x + \sqrt{3}}{x\sqrt{3} - 1}$:
\[
f^3(x) = \frac{-\frac{x + \sqrt{3}}{x\sqrt{3} - 1} - \sqrt{3}}{-\frac{x + \sqrt{3}}{x\sqrt{3} - 1}\sqrt{3} + 1}
\]
Numerator:
\begin{align*}
&-\frac{x + \sqrt{3}}{x\sqrt{3} - 1} - \sqrt{3} \\
&= \frac{-(x + \sqrt{3}) - \sqrt{3}(x\sqrt{3} - 1)}{x\sqrt{3} - 1} \\
&= \frac{-(x + \sqrt{3}) - x\cdot 3 + \sqrt{3}}{x\sqrt{3} - 1} \\
&= \frac{-(x + \sqrt{3}) - 3x + \sqrt{3}}{x\sqrt{3} - 1} \\
&= \frac{-x - \sqrt{3} - 3x + \sqrt{3}}{x\sqrt{3} - 1} \\
&= \frac{-4x}{x\sqrt{3} - 1}
\end{align*}
Denominator:
\begin{align*}
&-\frac{x + \sqrt{3}}{x\sqrt{3} - 1}\sqrt{3} + 1 \\
&= -\frac{(x + \sqrt{3})\sqrt{3}}{x\sqrt{3} - 1} + 1 \\
&= \frac{-(x\sqrt{3} + 3) + (x\sqrt{3} - 1)}{x\sqrt{3} - 1} \\
&= \frac{-(x\sqrt{3} + 3) + x\sqrt{3} - 1}{x\sqrt{3} - 1} \\
&= \frac{-3 - 1}{x\sqrt{3} - 1} \\
&= \frac{-4}{x\sqrt{3} - 1}
\end{align*}
So,
\[
f^3(x) = \frac{-4x}{-4} = x
\]

Thus, $f^3(x) = x$, so $f$ is of order $3$ under composition. Therefore,
\[
f^{2012}(x) = f^{2012 \bmod 3}(x)
\]
Since $2012 \div 3 = 670$ remainder $2$, $2012 \bmod 3 = 2$.

Therefore,
\[
\boxed{f^{2012}(x) = f^2(x) = -\frac{x + \sqrt{3}}{x\sqrt{3} - 1}}
\]

\end{document}