\documentclass{article}

\usepackage{amsmath}
\usepackage{amssymb}
\usepackage{amsthm}

\title{Week 14 Writing Problem}
\author{Michael Xie, \\
        Art of Problem Solving, \\
        Intermediate Algebra}
\date{\today}

\begin{document}

\maketitle

\section*{Problem}
The sequence $(a_n)$ is defined by $a_1 = \frac{1}{2}$ and
\[
  a_n = a_{n - 1}^2 + a_{n - 1}
\]
for all $n \ge 2.$

Prove that
\[
  \frac{1}{a_1 + 1} + \frac{1}{a_2 + 1} + \dots + \frac{1}{a_k + 1} < 2
\]
for all $k \ge 1.$

\section*{Solution}
Observe first that
\[
  a_{n+1} \;=\; a_n^2 + a_n
  \quad\Longrightarrow\quad
  a_{n+1}-a_n = a_n^2,
\]
so
\[
  \frac1{a_n}-\frac1{a_{n+1}}
  \;=\;
  \frac{a_{n+1}-a_n}{a_n\,a_{n+1}}
  \;=\;
  \frac{a_n^2}{a_n\,a_{n+1}}
  \;=\;
  \frac1{a_{n+1}}
  \;=\;
  \frac1{a_n+1}.
\]
Hence for each $n\ge1$,
\[
  \frac1{a_n+1}
  \;=\;
  \frac1{a_n}-\frac1{a_{n+1}},
\]
and the sum telescopes:
\[
  \sum_{n=1}^k \frac1{a_n+1}
  \;=\;
  \Bigl(\tfrac1{a_1}-\tfrac1{a_2}\Bigr)
  +\Bigl(\tfrac1{a_2}-\tfrac1{a_3}\Bigr)
  +\cdots+
  \Bigl(\tfrac1{a_k}-\tfrac1{a_{k+1}}\Bigr)
  \;=\;
  \frac1{a_1}-\frac1{a_{k+1}}.
\]
Since $a_1=\tfrac12$, this becomes
\[
  \sum_{n=1}^k \frac1{a_n+1}
  \;=\;
  2 \,-\, \frac1{a_{k+1}}
  \;<\;
  2,
\]
as claimed.

\section*{Conclusion}
The sequence $(a_n)$ is defined recursively, and we have shown that the sum of the series converges to a value less than 2. This demonstrates the power of telescoping series in simplifying complex recursive definitions.
\end{document}
